wip: add post-conditions for bignum.curve25519

code/experimental/curve25519/Hacl.Impl.Curve25519.Field51.fst
@@ -8,9 +8,10 @@ open Lib.Sequence
 open Lib.IntTypes
 open Lib.Buffer
 
-include Hacl.Spec.Curve25519.Field51.Definition
 include Hacl.Spec.Curve25519.Field51
+include Hacl.Spec.Curve25519.Field51.Definition
 
+module S = Hacl.Spec.Curve25519.Field51.Definition
 module ST = FStar.HyperStack.ST
 
 #reset-options "--z3rlimit 20"
@@ -28,7 +29,7 @@ let as_nat h e =
   let s2 = s.[2] in
   let s3 = s.[3] in
   let s4 = s.[4] in
-  as_nat5 (s0, s1, s2, s3, s4)
+  S.as_nat5 (s0, s1, s2, s3, s4)
 
 noextract
 val wide_as_nat: h:mem -> e:felem_wide -> GTot nat
@@ -39,10 +40,18 @@ let wide_as_nat h e =
   let s2 = s.[2] in
   let s3 = s.[3] in
   let s4 = s.[4] in
-  wide_as_nat5 (s0, s1, s2, s3, s4)
+  S.wide_as_nat5 (s0, s1, s2, s3, s4)
 
 noextract
-val felem_fits: h:mem -> f:felem -> m:scale64_5 -> Type0
+val fevalh: h:mem -> f:felem -> GTot S.felem
+let fevalh h f = (as_nat h f) % S.prime
+
+noextract
+val feval_wideh: h:mem -> f:felem_wide -> GTot S.felem
+let feval_wideh h f = (wide_as_nat h f) % S.prime
+
+noextract
+val felem_fits: h:mem -> f:felem -> m:S.scale64_5 -> Type0
 let felem_fits h f m =
   let s = as_seq h f in
   let s0 = s.[0] in
@@ -50,10 +59,10 @@ let felem_fits h f m =
   let s2 = s.[2] in
   let s3 = s.[3] in
   let s4 = s.[4] in
-  felem_fits5 (s0, s1, s2, s3, s4) m
+  S.felem_fits5 (s0, s1, s2, s3, s4) m
 
 noextract
-val felem_wide_fits: h:mem -> f:felem_wide -> m:scale128_5 -> Type0
+val felem_wide_fits: h:mem -> f:felem_wide -> m:S.scale128_5 -> Type0
 let felem_wide_fits h f m =
   let s = as_seq h f in
   let s0 = s.[0] in
@@ -61,7 +70,7 @@ let felem_wide_fits h f m =
   let s2 = s.[2] in
   let s3 = s.[3] in
   let s4 = s.[4] in
-  felem_wide_fits5 (s0, s1, s2, s3, s4) m
+  S.felem_wide_fits5 (s0, s1, s2, s3, s4) m
 
 
 inline_for_extraction
@@ -107,7 +116,9 @@ inline_for_extraction
 val set_zero:
   f:felem -> Stack unit
   (requires fun h -> live h f)
-  (ensures  fun h0 _ h1 -> modifies (loc f) h0 h1)
+  (ensures  fun h0 _ h1 ->
+    modifies (loc f) h0 h1 /\
+    as_nat h1 f == 0)
 let set_zero f =
   f.(0ul) <- u64 0;
   f.(1ul) <- u64 0;
@@ -120,14 +131,19 @@ val copy_felem:
     f1:felem
   -> f2:felem
   -> Stack unit
-    (requires fun h -> live h f1 /\ live h f2)
-    (ensures  fun h0 _ h1 -> modifies (loc f1) h0 h1)
+    (requires fun h ->
+      live h f1 /\ live h f2 /\ disjoint f1 f2)
+    (ensures  fun h0 _ h1 ->
+      modifies (loc f1) h0 h1 /\
+      as_nat h1 f1 == as_nat h0 f2)
 let copy_felem f1 f2 =
   f1.(size 0) <- f2.(size 0);
   f1.(size 1) <- f2.(size 1);
   f1.(size 2) <- f2.(size 2);
   f1.(size 3) <- f2.(size 3);
   f1.(size 4) <- f2.(size 4)
+
+#set-options "--max_fuel 0 --max_ifuel 0"
 
 val fadd:
     out:felem
@@ -141,9 +157,10 @@ val fadd:
     (ensures fun h0 _ h1 ->
       modifies (loc out) h0 h1 /\
       felem_fits h1 out (2, 4, 2, 2, 2) /\
-      as_nat h1 out == as_nat h0 f1 + as_nat h0 f2)
+      fevalh h1 out == S.fadd (fevalh h0 f1) (fevalh h0 f2))
 [@ CInline]
 let fadd out f1 f2 =
+  let h0 = ST.get () in
   let f10 = f1.(0ul) in
   let f20 = f2.(0ul) in
   let f11 = f1.(1ul) in
@@ -158,7 +175,13 @@ let fadd out f1 f2 =
   out.(1ul) <- f11 +! f21;
   out.(2ul) <- f12 +! f22;
   out.(3ul) <- f13 +! f23;
-  out.(4ul) <- f14 +! f24
+  out.(4ul) <- f14 +! f24;
+  let h1 = ST.get () in
+  assert (as_nat h1 out == as_nat h0 f1 + as_nat h0 f2);
+  FStar.Math.Lemmas.lemma_mod_plus_distr_l
+    (as_nat h0 f1) (as_nat h0 f2) S.prime;
+  FStar.Math.Lemmas.lemma_mod_plus_distr_r
+    (as_nat h0 f1 % S.prime) (as_nat h0 f2) S.prime
 
 val fsub:
     out:felem
@@ -171,7 +194,8 @@ val fsub:
       felem_fits h f2 (1, 2, 1, 1, 1))
     (ensures  fun h0 _ h1 ->
       modifies (loc out) h0 h1 /\
-      felem_fits h1 out (9, 10, 9, 9, 9))
+      felem_fits h1 out (9, 10, 9, 9, 9) /\
+      fevalh h1 out == S.fsub (fevalh h0 f1) (fevalh h0 f2))
 [@ CInline]
 let fsub out f1 f2 =
   let f10 = f1.(0ul) in
@@ -188,7 +212,8 @@ let fsub out f1 f2 =
   out.(1ul) <- f11 +! u64 0x3ffffffffffff8 -! f21;
   out.(2ul) <- f12 +! u64 0x3ffffffffffff8 -! f22;
   out.(3ul) <- f13 +! u64 0x3ffffffffffff8 -! f23;
-  out.(4ul) <- f14 +! u64 0x3ffffffffffff8 -! f24
+  out.(4ul) <- f14 +! u64 0x3ffffffffffff8 -! f24;
+  lemma_fsub (f10, f11, f12, f13, f14) (f20, f21, f22, f23, f24)
 
 val fmul:
     out:felem
@@ -201,7 +226,8 @@ val fmul:
       felem_fits h f2 (9, 10, 9, 9, 9))
     (ensures  fun h0 _ h1 ->
       modifies (loc out) h0 h1 /\
-      felem_fits h1 out (1, 2, 1, 1, 1))
+      felem_fits h1 out (1, 2, 1, 1, 1) /\
+      fevalh h1 out == S.fmul (fevalh h0 f1) (fevalh h0 f2))
 [@ CInline]
 let fmul out f1 f2 =
   let f10 = f1.(size 0) in
@@ -241,8 +267,14 @@ val fmul2:
     (ensures  fun h0 _ h1 -> modifies (loc out) h0 h1 /\
      (let out0 = gsub out 0ul 5ul in
       let out1 = gsub out 5ul 5ul in
+      let f10 = gsub f1 0ul 5ul in
+      let f11 = gsub f1 5ul 5ul in
+      let f20 = gsub f2 0ul 5ul in
+      let f21 = gsub f2 5ul 5ul in
       felem_fits h1 out0 (1, 2, 1, 1, 1) /\
-      felem_fits h1 out1 (1, 2, 1, 1, 1)))
+      felem_fits h1 out1 (1, 2, 1, 1, 1) /\
+      fevalh h1 out0 == S.fmul (fevalh h0 f10) (fevalh h0 f20) /\
+      fevalh h1 out1 == S.fmul (fevalh h0 f11) (fevalh h0 f21)))
 [@ CInline]
 let fmul2 out f1 f2 =
   let f10 = f1.(size 0) in
@@ -293,10 +325,11 @@ val fmul1:
     (requires fun h ->
       live h out /\ live h f1 /\
       felem_fits h f1 (9, 10, 9, 9, 9) /\
-      felem_fits1 f2 1)
+      S.felem_fits1 f2 1)
     (ensures  fun h0 _ h1 ->
       modifies (loc out) h0 h1 /\
-      felem_fits h1 out (1, 2, 1, 1, 1))
+      felem_fits h1 out (1, 2, 1, 1, 1) /\
+      fevalh h1 out == (fevalh h0 f1 * v f2) % S.prime)
 [@ CInline]
 let fmul1 out f1 f2 =
   let f10 = f1.(size 0) in
@@ -320,7 +353,8 @@ val fsqr:
       felem_fits h f (9, 10, 9, 9, 9))
     (ensures  fun h0 _ h1 ->
       modifies (loc out) h0 h1 /\
-      felem_fits h1 out (1, 2, 1, 1, 1))
+      felem_fits h1 out (1, 2, 1, 1, 1) /\
+      fevalh h1 out == S.fsqr (fevalh h0 f))
 [@ CInline]
 let fsqr out f =
   let f0 = f.(0ul) in
@@ -349,8 +383,12 @@ val fsqr2:
       modifies (loc out) h0 h1 /\
      (let out1 = gsub out 0ul 5ul in
       let out2 = gsub out 5ul 5ul in
+      let f1 = gsub f 0ul 5ul in
+      let f2 = gsub f 5ul 5ul in
       felem_fits h1 out1 (1, 2, 1, 1, 1) /\
-      felem_fits h1 out2 (1, 2, 1, 1, 1)))
+      felem_fits h1 out2 (1, 2, 1, 1, 1) /\
+      fevalh h1 out1 == S.fsqr (fevalh h0 f1) /\
+      fevalh h1 out2 == S.fsqr (fevalh h0 f2)))
 [@ CInline]
 let fsqr2 out f =
   let f10 = f.(0ul) in
@@ -365,7 +403,8 @@ let fsqr2 out f =
   let f23 = f.(8ul) in
   let f24 = f.(9ul) in
 
-  let ((o10,o11,o12,o13,o14),(o20,o21,o22,o23,o24)) = fsqr25 (f10,f11,f12,f13,f14) (f20,f21,f22,f23,f24) in
+  let ((o10,o11,o12,o13,o14),(o20,o21,o22,o23,o24)) =
+    fsqr25 (f10,f11,f12,f13,f14) (f20,f21,f22,f23,f24) in
   out.(size 0) <- o10;
   out.(size 1) <- o11;
   out.(size 2) <- o12;
@@ -386,7 +425,7 @@ val load_felem:
     (requires fun h -> live h u64s /\ live h f)
     (ensures  fun h0 _ h1 -> modifies (loc f) h0 h1)
 let load_felem f u64s =
-  let f0l = u64s.(0ul) &. mask51 in
+  let f0l = u64s.(0ul) &. S.mask51 in
   let f0h = u64s.(0ul) >>. 51ul in
   let f1l = (u64s.(1ul) &. u64 0x3fffffffff) <<. 13ul in
   let f1h = u64s.(1ul) >>. 38ul in
